HMAC: Non incremental pure specification update for secrecy of the input lengths

crypto_hst/hmac/HMAC.Pure.fst
@@ -5,68 +5,76 @@ open Hacl.UInt32
 open Hacl.SBuffer
 open Hacl.Operations.Pure
 
+module U8 = FStar.UInt8
+module S8 = Hacl.UInt8
+module U32 = FStar.UInt32
+module S32 = Hacl.UInt32
+module U64 = FStar.UInt64
+module S64 = Hacl.UInt64
+module SB = Hacl.SBuffer
+
 
 
 (* Define base types *)
+let u8 = FStar.UInt8.t
+let s8 = Hacl.UInt8.t
 let u32 = FStar.UInt32.t
-let uint32s = Hacl.SBuffer.u32s
-let bytes = Seq.seq Hacl.UInt8.t
+let s32 = Hacl.UInt32.t
+let uint32s = Seq.seq s32
+let bytes = Seq.seq s8
 
 
 (* Define algorithm parameters *)
 let hash = Hash.Sha256.Pure.sha256
-let hl = Hash.Sha256.Pure.hl
-let bl = Hash.Sha256.Pure.bl
-let hashsize = hl
-let blocksize = bl
+let hashsize = Hash.Sha256.Pure.hl
+let blocksize = Hash.Sha256.Pure.bl
+let hl = hashsize
+let bl = blocksize
 
 
-(* Define operators *)
-let op_At_Plus = FStar.UInt32.add
-let op_At_Subtraction = FStar.UInt32.sub
-
+let u8_to_s8 = Hacl.Cast.uint8_to_sint8
+let u32_to_s32 = Hacl.Cast.uint32_to_sint32
 
 
 (* Define a function to wrap the key length after bl bits *)
-let wrap_key (key:bytes) (keylen:u32{Seq.length key = v keylen}) : GTot (okey:bytes{Seq.length okey = v bl}) =
-  if gt keylen bl then
+let wrap_key (key:bytes) (keylen:s32{Seq.length key = S32.v keylen}) : GTot (okey:bytes{Seq.length okey = U32.v bl}) =
+  if S32.v keylen > U32.v bl then
     let okey = hash key keylen in
-    Seq.append okey (Seq.create (v bl - v hl) 0uy)
+    Seq.append okey (Seq.create (U32.v bl - U32.v hl) (u8_to_s8 0uy))
   else
-    Seq.append key (Seq.create (v bl - v keylen) 0uy)
+    Seq.append key (Seq.create (U32.v bl - S32.v keylen) (u8_to_s8 0uy))
 
 
 (* Define the internal function *)
 val hmac_core : (key     :bytes) ->
-                (keylen  :u32{Seq.length key = v keylen}) ->
+                (keylen  :s32{Seq.length key = S32.v keylen}) ->
                 (data    :bytes) ->
-                (datalen :u32{Seq.length data = v datalen /\ v bl + v datalen < pow2 32})
-  -> GTot (mac:bytes{Seq.length mac = v hl})
+                (datalen :s32{Seq.length data = S32.v datalen /\ U32.v bl + S32.v datalen < pow2 32})
+  -> GTot (mac:bytes{Seq.length mac = U32.v hl})
 
 let hmac_core key keylen data datalen =
-  
+
   (* Define ipad and opad *)
-  let ipad = Seq.create (v bl) 0x36uy in
-  let opad = Seq.create (v bl) 0x5cuy in
-  
+  let ipad = Seq.create (U32.v bl) (u8_to_s8 0x36uy) in
+  let opad = Seq.create (U32.v bl) (u8_to_s8 0x5cuy) in
+
   (* Step 1: make sure the key has the proper length *)
   let okey = wrap_key key keylen in
 
   (* Step 2: xor "result of step 1" with ipad *)
   let s2 = xor_bytes ipad okey bl in
-  
+
   (* Step 3: append data to "result of step 2" *)
   let s3 = Seq.append s2 data in
-  
+
   (* Step 4: apply H to "result of step 3" *)
-  let s4 = hash s3 (bl @+ datalen) in
- 
+  let s4 = hash s3 (u32_to_s32 bl +^ datalen) in
+
   (* Step 5: xor "result of step 1" with opad *)
   let s5 = xor_bytes okey opad bl in
-  
+
   (* Step 6: append "result of step 4" to "result of step 5" *)
   let s6 = Seq.append s5 s4 in
 
   (* Step 7: apply H to "result of step 6" *)
-  hash s6 (bl @+ hl)
-  
+  hash s6 (u32_to_s32 bl +^ u32_to_s32 hl)
